\chapter{boundary line}

\section{derive surface charge density}
\[
z=\frac{\zeta}{2}+\frac{1}{2\zeta}
\]

\begin{align*}
 \sigma(z) &= \left| \frac{dw}{dz} \right| = \left| \frac{dw}{\df\zeta} \frac{\df \zeta}{\df z} \right| \\
\frac{\df\zeta}{\df z} &= \left( \frac{\df z}{\df\zeta} \right)^{-1}, \quad \frac{\df z}{\df\zeta} = \frac{1}{2} \left( 1 - \frac{1}{\zeta^2} \right) \\
\left. 1 - \frac{1}{\zeta^2} \right|_{\zeta=e^{\im \theta}} &= \left| \frac{\zeta^2 - 1}{\zeta^2} \right| = \left| \frac{e^{i2\theta} - 1}{e^{i2\theta}} \right| \\
\left| \frac{\df z}{\df\zeta} \right| &= \frac{1}{2} \left| e^{i2\theta} - 1 \right| = \frac{1}{2} \sqrt{(\cos 2\theta - 1)^2 + \sin^2 2\theta} \\
&= \frac{1}{2} \sqrt{\cos^2 2\theta + \sin^2 2\theta + 1 - 2\cos 2\theta} \\
&= \frac{1}{2} \sqrt{2 - 2\cos 2\theta} = \frac{\sqrt{2}}{2} \sqrt{1 - \cos 2\theta} \\
&= \frac{\sqrt{2}}{2} \sqrt{2\sin^2 \theta} = \sin \theta \\
\left| \frac{\df \zeta}{\df z} \right| &= \frac{1}{\sin \theta}
\end{align*}

\[
w(\zeta) = \frac{q_t}{2\pi \epsilon_0} \im \left[ \log(\zeta - \zeta_0) - i \log\left(\frac{1}{\zeta} - \overline{\zeta_0}\right) \right]
\]
define $\frac{q_t}{2\pi \epsilon_0}\im\coloneqq 1$
\[
\frac{dw}{d\zeta} \sim  \frac{1}{\zeta - \zeta_0} - \frac{1}{\frac{1}{\zeta} - \overline{\zeta_0}} \cdot \frac{-1}{\zeta^2} 
\]

\[
=  \frac{1}{\zeta - \zeta_0} + \frac{1}{\zeta + \zeta^2\overline{\zeta_0}} 
\]

\[
\text{at } \zeta = e^{i\theta}, \quad z = \frac{\zeta + \frac{1}{\zeta}}{2} = \cos \theta =x
\]
$\theta\in(0,\pi)$ and $x\in(1,-1)$ 
\[
\Rightarrow \sigma(\theta) = \left| \frac{dw}{d\zeta} \frac{d\zeta}{dz} \right| (\theta)= \frac{q_t}{2\pi \epsilon_0}\left| \frac{1}{e^{i\theta} - \zeta_0} + \frac{1}{e^{i\theta} + e^{i2\theta}\overline{\cdot \zeta_0}} \right| \cdot \frac{1}{\sin \theta}
\]
in $x$, and $y\equiv0$
\[
\Rightarrow \sigma(x) = \frac{q_t}{2\pi \epsilon_0}\left| \frac{1}{x+\im\sqrt{1-x^2} - \zeta_0} + \frac{1}{x+\im\sqrt{1-x^2} + (x+\im\sqrt{1-x^2})^2\overline{\cdot \zeta_0}} \right| \cdot \frac{1}{\sqrt{1-x^2}}
\]




\section{$h$}
$w(z)$ $w_1$,$w_2$\\
$w_1$
\[
w = i \log \left( z + \sqrt{z^2 - 1} - \zeta_0 \right) - i \log \left( \frac{1}{z + \sqrt{z^2 - 1}} - \overline{\zeta_0} \right)
\]
\[
\frac{\partial w_1}{\partial z} = \frac{1}{z + \sqrt{z^2 - 1} - \zeta_0} \cdot \left( 1 + \frac{z}{\sqrt{z^2 - 1}} \right)
\]
\[
= \frac{1}{\sqrt{z^2 - 1}} \cdot \frac{z + \sqrt{z^2 - 1}}{z + \sqrt{z^2 - 1} - \zeta_0}
\]
\( z = x \), \( x \in (0,1) \), $\zeta_0\coloneqq-a\im$
\[
\frac{\partial w_1}{\partial z} \Bigg|_{z=x} = \frac{1}{\im\sqrt{1 - x^2}} \cdot \frac{x + i \sqrt{1 - x^2}}{x + i \left( a + \sqrt{1 - x^2} \right)}
\]
\[
\left| \frac{\partial w_1}{\partial z} \right|_{z=x}= \frac{1}{\sqrt{1 - x^2}} \cdot \frac{\left|x + i \sqrt{1 - x^2}\right|}{\sqrt{x^2 + a^2 + \left( \sqrt{1 - x^2} \right)^2 + 2a \sqrt{1 - x^2}}}
\]

\[
\left| \frac{\partial w_1}{\partial z} \right|_{z=x} = \frac{1}{\sqrt{1 - x^2}} \cdot \frac{1}{a^2 + 1 + 2a \sqrt{1 - x^2}}
\]
as
\[
a^2 + 1 + 2a \sqrt{1 - x^2}>a^2 + 1 + 2a=(a+1)^2\geq 0
\]
$w_2$\\
\[
\frac{\partial w_2}{\partial z} = -i \cdot \frac{1}{\frac{1}{z + \sqrt{z^2 - 1}} - \overline{\zeta_0}} \cdot \left(\frac{1}{z+\sqrt{z^2 - 1}}\right)'
\]
\[= -i \cdot \frac{z + \sqrt{z^2 - 1}}{1 - \overline{\zeta_0}\left(z + \sqrt{z^2 - 1}\right)} \cdot \frac{-1}{\left(z+\sqrt{z^2 - 1}\right)^2} \cdot \left( 1 + \frac{z}{\sqrt{z^2 - 1}} \right)
\]
\[
= \frac{i}{\sqrt{z^2 - 1}} \cdot \frac{z + \sqrt{z^2 - 1}}{1 - a i \left( z + \sqrt{z^2 - 1} \right)}
\]
 \( z = x \)
\[
\frac{\partial w_2}{\partial z} \Bigg|_{z=x} = \frac{\im}{\im\sqrt{1 - x^2}} \cdot \frac{1}{1 - a i x - a \im\im \sqrt{1 - x^2}}
\]

\[
\left| \frac{\partial w_2}{\partial z} \right|_{z=x}= \frac{1}{\sqrt{1 - x^2}} \cdot \frac{1}{\sqrt{(1 + a \sqrt{1 - x^2})^2 + (a x)^2}}
\]

\[
\left| \frac{\partial w_2}{\partial z} \right|_{z=x} = \frac{1}{\sqrt{1 - x^2}} \cdot \frac{1}{1 + a^2 + 2 a \sqrt{1 - x^2}}
\]
hence
\[
\left|\frac{\df w}{\df z}\right|_{z=x}=\left|\frac{\df w_1}{\df z}+\frac{\df w_2}{\df z}\right|_{z=x} = \frac{2}{\sqrt{1 - x^2}} \cdot \frac{1}{1 + a^2 + 2 a \sqrt{1 - x^2}}
\]
that is, in $z$, the charge density on the upper slit
\[
\sigma\sim \frac{2}{\sqrt{1 - x^2}} \cdot \frac{1}{1 + a^2 + 2 a \sqrt{1 - x^2}}
\]
\begin{figure}[H]
    \centering
    \includegraphics[width=0.85\linewidth]{Figs/surface charge density.jpg}
    \caption{\small surface charge density, $x\in(-0.99, 0.99)$, at the boundary area, the value goes to $\infty$, hence omitted}
    \label{fig:enter-label}
\end{figure}
and
\[
\int \sigma \sim \arctan \sqrt{1-x^2}
\]
\pagebreak
