\subsection{Derivation Using the Divergence Theorem}
\hspace{0em}\indent We next try the divergence theorem. The variation in the electric field $\delta E_e$ is:
\begin{equation*}
    \delta \mathcal{E}_e=+\delta\left(-\frac{\epsilon}{2}\int_{\mathbb{R}^2\setminus\Omega}|E|^2 \df S
\right)=\int_{\delta\partial\Omega}...-\frac{\epsilon}{2}\int_{\mathbb{R}^2\setminus\Omega}\delta|E|^2 \df S\simeq-\frac{\epsilon}{2}\int_{\mathbb{R}^2\setminus\Omega}2\vec{E}\cdot\delta\vec{E} \df S
\end{equation*}
Let $\vec{G}\coloneqq\vec{E}\delta V$, $V$ is the voltage.
\begin{equation*}
    \begin{split}
    \delta \mathcal{E}_e&=-\epsilon\int_{\mathbb{R}^2\setminus\Omega}\vec{E}\cdot\delta(-\nabla V) \df S=\epsilon\int_{\mathbb{R}^2\setminus\Omega}\vec{E}\cdot(\nabla \delta V) \df S
    \end{split}
    \end{equation*}
Use $\nabla\cdot(\vec{A}\phi)=\phi\nabla\cdot\vec{A}+\vec{A}\cdot\nabla\phi$
\begin{equation}\label{eqn:div_find_0}
    \begin{split}
    \delta \mathcal{E}_e&=\epsilon\int_{\mathbb{R}^2\setminus\Omega}\nabla\cdot(\vec{E}\, \delta V) -\delta V \eqnmarkbox[black]{node1}{\nabla\cdot\vec{E}}\df S\\
    &=\epsilon\int_{\mathbb{R}^2\setminus\Omega}\nabla\cdot(\vec{E}\, \delta V) \df S \xlongequal[ ]{\text{div thm}}\oint_{...}\vec{G}\cdot\hat{n}\df l \epsilon=\int_{\partial \Omega}...+\eqnmarkbox[black]{node2}{\int_{r\rightarrow\infty}\vec{E}}\cdot\hat{n}\, \delta V\df l\\
    &=\epsilon\int_{\partial\Omega}\vec{E}\cdot\hat{n}\, \delta V \df l=\sigma\int_{\partial \Omega}\delta V \df l\\
    \end{split}
\end{equation}
\annotate[yshift=1em]{above, right, label above}{node1}{$\nabla \cdot \vec{E}|_{\mathbb{R}^2\setminus \Omega}= 0$}
\annotate[yshift=1em]{above, right, label above}{node2}{$=0,\vec{E}|_{r\rightarrow\infty}\rightarrow 0$}

\vspace{-1em}
\noindent Equation (\ref{eqn:ed.line}) shows $\vec{E}|_{\partial \Omega}=\sigma/\epsilon\hat{n}$. To have the desired result, we expect
\[\int_{\partial \Omega} \delta V \df l =-\frac{\sigma}{2\epsilon}\int_{\delta \partial \Omega}\df l\Longrightarrow\delta V = -\frac{\sigma}{2\epsilon}\delta l\]
Moreover\footnote{Refer to \cite{Griffiths_2017}, equation (2.50).}, \vspace{0.5em}
\[\delta V =  -\frac{1}{2}(\vec{E}_{above}+\eqnmarkbox[black]{node1}{{\vec{E}_{below}}})\cdot \delta \vec{l}=-\frac{\vec{E}_{above}}{2}\delta \vec{l}=-\frac{\sigma}{2\epsilon}\hat{n}\cdot \delta \vec{l}\]
\annotate[yshift=1.0em]{above, right, label above}{node1}{$=0$}

\vspace{-1.5em}
\noindent Since $V=\int \vec{E}\Longrightarrow \delta V \sim \vec{E}_{average}\cdot\delta\vec{d}$. Let $\delta l=\hat{n}\cdot\delta\vec{l}$, We derive the wanted equation,
